progress on merging

LeanStlc/BoolNatTerm.lean
@@ -1,9 +1,12 @@
 import LeanStlc.NatTerm
 import LeanStlc.BoolTerm
 
-namespace BoolNatTerm
+open LeanSubst
 
-modular (name := `BoolNatTerm) (imports := #[`BoolTerm.BoolTerm, `NatExt.NatTerm])
+
+modular (name := `BoolNatTerm) (imports := #[`BoolTerm, `NatTerm])
+
+  namespace BoolNatTerm
 
   inductive Ty extends NatExt.Ty, BoolTerm.Ty
 
@@ -75,6 +78,214 @@ modular (name := `BoolNatTerm) (imports := #[`BoolTerm.BoolTerm, `NatExt.NatTerm
 
   mod def apply_id extends NatExt.apply_id, BoolTerm.apply_id
 
-  set_option trace.Modular true in
   mod def apply_stable extends NatExt.apply_stable, BoolTerm.apply_stable
-  #check apply_stable._proof_2
+
+
+  @[instance]
+  mod def SubstMapStable_Term extends NatExt.SubstMapStable_Term, BoolTerm.SubstMapStable_Term
+
+  @[simp]
+  mod def apply_compose extends NatExt.apply_compose, BoolTerm.apply_compose
+
+  @[instance]
+  mod def SubstMapCompose_Term extends NatExt.SubstMapCompose_Term, BoolTerm.SubstMapCompose_Term
+
+  mod def to_ren_is_var extends NatExt.to_ren_is_var,BoolTerm.to_ren_is_var
+  mod def ren_subst_apply_eq_lift extends NatExt.ren_subst_apply_eq_lift, BoolTerm.ren_subst_apply_eq_lift
+  mod def ren_subst_apply_eq extends NatExt.ren_subst_apply_eq, BoolTerm.ren_subst_apply_eq
+
+-- modular (imports := #[`Term]) (name := `ParRed)
+  inductive ParRed extends NatExt.ParRed, BoolTerm.ParRed where
+
+  attribute [grind] ParRed
+
+  namespace ParRed
+
+  @[grind .]
+  mod def refl extends NatExt.ParRed.refl, BoolTerm.ParRed.refl
+
+  @[grind .]
+  mod def subst extends NatExt.ParRed.subst, BoolTerm.ParRed.subst
+
+  @[grind .]
+  mod def subst_action extends NatExt.ParRed.subst_action, BoolTerm.ParRed.subst_action
+
+  @[grind .]
+  mod def subst_red_lift extends NatExt.ParRed.subst_red_lift, BoolTerm.ParRed.subst_red_lift
+
+  theorem hsubst {t t' : Term} {σ σ' : LeanSubst.Subst Term} :
+    (∀ x, ActionRed ParRed (σ x) (σ' x)) ->
+    ParRed t t' ->
+    ParRed t[σ] t'[σ']
+  := sorry
+  add_mapping NatExt.ParRed.hsubst => ParRed.hsubst
+  add_mapping BoolTerm.ParRed.hsubst => ParRed.hsubst
+
+
+  @[simp, grind]
+  mod def complete extends NatExt.ParRed.complete, BoolTerm.ParRed.complete
+
+  -- mod def triangle extends NatExt.ParRed.triangle, BoolTerm.ParRed.triangle
+
+  theorem triangle {t s : Term} : ParRed t s -> ParRed s (complete t) := sorry
+
+  add_mapping NatExt.ParRed.triangle => ParRed.triangle
+  add_mapping BoolTerm.ParRed.triangle => ParRed.triangle
+
+  mod def instSubstitutiveTerm extends NatExt.ParRed.instSubstitutiveTerm, BoolTerm.ParRed.instSubstitutiveTerm
+
+  mod def instHasTriangleTerm extends NatExt.ParRed.instHasTriangleTerm, BoolTerm.ParRed.instHasTriangleTerm
+
+  end ParRed
+
+-- modular (name := `Red) (imports := #[`ParRed])
+  inductive Red extends NatExt.Red, BoolTerm.Red
+
+
+  attribute [grind] Red
+
+  namespace Red
+
+  mod def subst extends NatExt.Red.subst, BoolTerm.Red.subst
+
+  @[grind .]
+  mod def seq_implies_par extends NatExt.Red.seq_implies_par, BoolTerm.Red.seq_implies_par
+
+  @[grind .]
+  mod def seqs_implies_pars extends NatExt.Red.seqs_implies_pars, BoolTerm.Red.seqs_implies_pars
+  mod def par_implies_seqs extends NatExt.Red.par_implies_seqs, BoolTerm.Red.par_implies_seqs
+  mod def pars_implies_seqs extends NatExt.Red.pars_implies_seqs, BoolTerm.Red.pars_implies_seqs
+  mod def pars_action_lift extends NatExt.Red.pars_action_lift, BoolTerm.Red.pars_action_lift
+  mod def seqs_action_lift extends NatExt.Red.seqs_action_lift, BoolTerm.Red.seqs_action_lift
+  mod def seqs_action_destruct extends NatExt.Red.seqs_action_destruct, BoolTerm.Red.seqs_action_destruct
+  mod def pars_action_iff_seqs_action extends NatExt.Red.pars_action_iff_seqs_action, BoolTerm.Red.pars_action_iff_seqs_action
+
+  mod def subst_action extends NatExt.Red.subst_action, BoolTerm.Red.subst_action
+  @[grind .]
+  mod def subst_red_lift extends NatExt.Red.subst_red_lift, BoolTerm.Red.subst_red_lift
+
+  mod def subst_arg extends NatExt.Red.subst_arg, BoolTerm.Red.subst_arg
+
+  mod def confluence extends NatExt.Red.confluence, BoolTerm.Red.confluence
+
+  mod def instSubstitutiveTerm extends NatExt.Red.instSubstitutiveTerm, BoolTerm.Red.instSubstitutiveTerm
+
+  mod def instHasConfluenceTerm extends NatExt.Red.instHasConfluenceTerm, BoolTerm.Red.instHasConfluenceTerm
+
+  -- TODO fix perf issue here
+  -- mod def preservation_of_neutral_step extends NatExt.Red.preservation_of_neutral_step, BoolTerm.Red.preservation_of_neutral_step
+
+  -- Bandaid fix
+  theorem preservation_of_neutral_step : Neutral t -> Red t t' -> Neutral t' := sorry
+  add_mapping NatExt.Red.preservation_of_neutral_step => preservation_of_neutral_step
+  add_mapping BoolTerm.Red.preservation_of_neutral_step => preservation_of_neutral_step
+
+  mod def preservation_of_neutral extends NatExt.Red.preservation_of_neutral, BoolTerm.Red.preservation_of_neutral
+
+  end Red
+
+  inductive Typing extends NatExt.Typing, BoolTerm.Typing
+
+  notation:170 Γ:170 " ⊢ " t:170 " : " A:170 => Typing Γ t A
+
+  attribute [grind .] Typing.var Typing.app Typing.lam Typing.zero Typing.succ Typing.natRec Typing.true Typing.false Typing.ite
+
+  mod def typing_renaming_lift extends NatExt.typing_renaming_lift, BoolTerm.typing_renaming_lift
+
+  mod def typing_weaken extends NatExt.typing_weaken, BoolTerm.typing_weaken
+
+  mod def typing_subst_lift extends NatExt.typing_subst_lift, BoolTerm.typing_subst_lift
+
+  mod def typing_subst extends NatExt.typing_subst, BoolTerm.typing_subst
+
+  mod def typing_beta extends NatExt.typing_beta, BoolTerm.typing_beta
+
+  mod def preservation_step extends NatExt.preservation_step, BoolTerm.preservation_step where
+    finally
+      all_goals grind (splits := 0) only
+
+  mod def preservation extends NatExt.preservation, BoolTerm.preservation
+
+  deriving instance DecidableEq for Ty
+
+  add_mapping NatExt.instDecidableEqTy => instDecidableEqTy
+  add_mapping BoolTerm.instDecidableEqTy => instDecidableEqTy
+
+  mod def is_arrow extends NatExt.is_arrow, BoolTerm.is_arrow
+
+  -- @[simp]
+  -- mod def infer extends NatExt.infer, BoolTerm.infer
+
+  -- currently fails with a weird unification error: two (synthetic opaque) mvars refuse to unify with a `readOnlyMVarWithBiggerLCtx` trace.
+  -- mod def extends NatExt.infer_sound, BoolTerm.infer_sound
+
+  -- modular (name := `Progress) (imports := #[`Red, `Typing])
+  @[grind]
+  mod def Term.is_lam extends NatExt.Term.is_lam, BoolTerm.Term.is_lam
+
+  inductive Value extends NatExt.Value, BoolTerm.Value
+
+  mod def value_sound extends NatExt.value_sound, BoolTerm.value_sound where
+    finally
+      all_goals grind (splits := 0) only
+
+  inductive VarSpine extends NatExt.VarSpine, BoolTerm.VarSpine where
+
+  mod def var_spine_not_lam extends NatExt.var_spine_not_lam, BoolTerm.var_spine_not_lam
+
+  mod def progress extends NatExt.progress, BoolTerm.progress where
+    finally
+      all_goals
+        intros
+        rename_i h
+        cases h
+        contradiction
+
+modular (name := `Part2) (imports := #[`BoolNatTerm])
+
+  inductive SnHeadRed extends NatExt.SnHeadRed, BoolTerm.SnHeadRed
+  infix:80 " ~>sn " => SnHeadRed
+
+  mod def SnHeadRed.red_compatible extends NatExt.SnHeadRed.red_compatible, BoolTerm.SnHeadRed.red_compatible where
+    finally
+      all_goals intros;contradiction
+
+  namespace SN
+  mod def subterm_ite extends BoolTerm.SN.subterm_ite
+  mod def subterm_natRec extends NatExt.SN.subterm_natRec
+  mod def subterm_app extends NatExt.SN.subterm_app, BoolTerm.SN.subterm_app
+  mod def lam extends NatExt.SN.lam, BoolTerm.SN.lam
+
+  mod def neutral_app extends NatExt.SN.neutral_app, BoolTerm.SN.neutral_app
+
+  mod def neutral_ite extends BoolTerm.SN.neutral_ite where finally
+    all_goals intros; contradiction
+
+  mod def neutral_nrec extends NatExt.SN.neutral_nrec where finally
+    all_goals intros; contradiction
+
+  mod def weak_head_expansion extends NatExt.SN.weak_head_expansion, BoolTerm.SN.weak_head_expansion
+
+  mod def red_app_preservation extends NatExt.SN.red_app_preservation, BoolTerm.SN.red_app_preservation
+
+  mod def backward_closure_app extends NatExt.SN.backward_closure_app, BoolTerm.SN.backward_closure_app
+
+  mod def backward_closure_ite extends BoolTerm.SN.backward_closure_ite  where finally
+    all_goals intros; contradiction
+
+  mod def backward_closure_nrec extends NatExt.SN.backward_closure_nrec  where finally
+    all_goals intros; contradiction
+
+  mod def true_expansion  extends BoolTerm.SN.true_expansion  where finally
+    all_goals intros; contradiction
+  mod def false_expansion extends BoolTerm.SN.false_expansion  where finally
+    all_goals intros; contradiction
+
+  mod def zero_expansion extends NatExt.SN.zero_expansion where finally
+    all_goals intros; contradiction
+  mod def succ_expansion extends NatExt.SN.succ_expansion where finally
+    all_goals intros; contradiction
+
+  mod def backward_closure extends NatExt.SN.backward_closure, BoolTerm.SN.backward_closure
+
+  end SN
